Add Haskell parser and examples

src/Instances.hs
@@ -1,0 +1,62 @@
+{-# OPTIONS_GHC -Wno-orphans #-}
+
+module Instances where
+
+import Data.List
+import Infer
+
+toList :: World -> List String -> List String
+toList Nil        = id
+toList (Snoc w a) = toList w . (a:)
+
+instance Show World where
+  show w = intercalate " " (Prelude.map ('?':) (toList w []))
+
+instance Show Exp where
+  showsPrec p e =
+    case e of
+      Var x         -> showString x
+      Infer.True    -> showString "true"
+      Infer.False   -> showString "false"
+      Ifte e1 e2 e3 -> showParen (p > 0) $
+                         showString "if " .
+                         showsPrec 0 e1 .
+                         showString " then ".
+                         showsPrec 0 e2 .
+                         showString " else ".
+                         showsPrec 0 e3
+      Absu x e1     -> showParen (p > 0) $
+                         showString "\\" .
+                         showString x .
+                         showString ". " .
+                         showsPrec 0 e1
+      Abst x t e1   -> showParen (p > 0) $
+                         showString "\\" .
+                         showString x .
+                         showString ":" .
+                         showsPrec 0 t .
+                         showString ". " .
+                         showsPrec 0 e1
+      App e1 e2     -> showParen (p > 1) $
+                         showsPrec 1 e1 .
+                         showString " " .
+                         showsPrec 2 e2
+
+instance Show Ty where
+  showsPrec p t =
+    case t of
+      Bool0         -> showString "bool"
+      Func0 t1 t2   -> showParen (p > 0) $
+                         showsPrec 1 t1 .
+                         showString " -> " .
+                         showsPrec 0 t2
+
+instance Show OTy where
+  showsPrec p t =
+    case t of
+      Evar alpha _ -> showString ('?':alpha)
+      Bool         -> showString "bool"
+      Func t1 t2   -> showParen (p > 0) $
+                        showsPrec 1 t1 .
+                        showString " -> " .
+                        showsPrec 0 t2
