src/Main.hs
@@ -1,0 +1,62 @@
+module Main where
+
+import Control.Exception
+import Control.Monad
+import Data.Semigroup ((<>))
+import Options.Applicative
+import System.Exit
+
+import Infer (Exp, Result(..), ground_expr, infer)
+import Instances ()
+import Parser (parse)
+
+optionsParser :: Parser String
+optionsParser =
+  argument str
+  (metavar "FILENAME" <>
+   help "Path to the file to type check")
+
+parserInfo :: ParserInfo String
+parserInfo =
+  info
+  (optionsParser <**> helper)
+  (fullDesc
+    <> progDesc "Typecheck FILENAME"
+    <> header "em - a typechecker for lambdabool" )
+
+doRead :: String -> IO String
+doRead path = handle h $ readFile path
+  where
+    h :: IOException -> IO String
+    h _ = putStrLn "Error: Unable to read the file." >>
+          exitWith (ExitFailure 1)
+
+doParse :: String -> IO Exp
+doParse content =
+  case parse content of
+    Left e -> do
+      putStrLn "Parsing failed:"
+      print e
+      exitWith (ExitFailure 1)
+    Right e -> do
+      putStr "Desugared exp: "
+      print e
+      return e
+
+doInfer :: Exp -> IO ()
+doInfer e =
+  case infer e of
+    Just r@(MkResult w ot _oe) -> do
+      putStr ("Unconstrained: ")
+      print w
+      putStr ("Inferred type: ")
+      print ot
+      putStr ("Reconstructed: ")
+      print (ground_expr r)
+
+    Nothing -> putStrLn "Inference failed"
+
+main :: IO ()
+main =
+  execParser parserInfo >>=
+  (doRead >=> doParse >=> doInfer)
