src/Parser.hs
@@ -1,0 +1,102 @@
+{-# OPTIONS_GHC -Wno-missing-signatures #-}
+
+module Parser where
+
+import Text.Parsec
+import qualified Text.Parsec.Token as P
+import Text.Parsec.Language (haskellDef)
+import Text.Parsec.String (Parser)
+
+import Infer
+
+lambdabooldef :: P.LanguageDef st
+lambdabooldef =
+  haskellDef
+  { P.reservedOpNames =
+    ["->",".",":","=","\\"]
+  , P.reservedNames   =
+    ["bool"
+    ,"else"
+    ,"false"
+    ,"if"
+    ,"in"
+    ,"let"
+    ,"then"
+    ,"true"
+    ]
+  }
+
+lexer       = P.makeTokenParser lambdabooldef
+parens      = P.parens lexer
+braces      = P.braces lexer
+identifier  = P.identifier lexer
+reserved    = P.reserved lexer
+reservedOp  = P.reservedOp lexer
+whiteSpace  = P.whiteSpace lexer
+
+-- Desugar let expressions into lambdas
+elet :: String -> Exp -> Exp -> Exp
+elet x e1 e2 = App (Absu x e2) e1
+
+primTy :: Parser Ty
+primTy = parens ty <|> Bool0 <$ reserved "bool"
+
+ty :: Parser Ty
+ty = chainr1 primTy (Func0 <$ reservedOp "->")
+
+varExpr :: Parser Exp
+varExpr = Var <$> identifier
+
+boolLitExpr :: Parser Exp
+boolLitExpr =
+  Infer.True  <$ reserved "true" <|>
+  Infer.False <$ reserved "false"
+
+ifteExpr :: Parser Exp
+ifteExpr =
+  Ifte
+  <$  reserved "if"
+  <*> expr
+  <*  reserved "then"
+  <*> expr
+  <*  reserved "else"
+  <*> expr
+
+lambdaExpr :: Parser Exp
+lambdaExpr = do
+  reservedOp "\\"
+  x <- identifier
+  (Absu x
+   <$ reservedOp "."
+   <*> expr
+   <|>
+   Abst x
+   <$ reservedOp ":"
+   <*> ty
+   <*  reservedOp "."
+   <*> expr)
+
+letExpr :: Parser Exp
+letExpr =
+  elet
+  <$  reserved "let"
+  <*> identifier
+  <*  reservedOp "="
+  <*> expr
+  <*  reserved "in"
+  <*> expr
+
+expr :: Parser Exp
+expr = foldl1 App <$> many1 primExpr
+
+primExpr :: Parser Exp
+primExpr =
+  parens expr
+  <|> varExpr
+  <|> boolLitExpr
+  <|> ifteExpr
+  <|> letExpr
+  <|> lambdaExpr
+
+parse :: String -> Either ParseError Exp
+parse = Text.Parsec.parse (whiteSpace >> expr) "<stdin>"
